

Relativity Lecture 1 Notes.

Suppose we have 2 coordinate systems:

—————→ A (x, t) B is moving with velocity v relative to A.

—————→ B (x', t') In B's perspective, A is moving with velocity $-v$ w.r.t B.

Assuming the (x, t) & (x', t') coordinate system is linearly related, we have the following.

$$\begin{cases} x' = \gamma(v)(x - vt) & \textcircled{1} \rightarrow \\ x = \gamma(v)(x' + vt') & \textcircled{2} \end{cases}$$

$$\frac{x}{\gamma} - vt' = x'$$

From ①: $\frac{x'}{\gamma} + vt = x$ ③

$$\frac{x}{\gamma} - \gamma x + \gamma vt = vt'$$

③ = ② $\frac{x'}{\gamma} + vt = \gamma(x' + vt')$

$$\frac{x'}{\gamma^2} + \frac{v}{\gamma}t = x' + vt'$$

$$\frac{v}{\gamma}t = \left(1 - \frac{1}{\gamma^2}\right)x' + vt'$$

$$t = \frac{\gamma}{v} \left(1 - \frac{1}{\gamma^2}\right)x' + \frac{\gamma}{v}vt'$$

$$= \frac{\gamma}{v} \left(1 - \frac{1}{\gamma^2}\right)x' + \gamma t'$$

$$t = \gamma \left[\frac{1}{v} \left(1 - \frac{1}{\gamma^2}\right)x' + t' \right]$$

$$\frac{\gamma^2 - 1}{\gamma^2}$$

$$\frac{\frac{1}{A^2} - 1}{\frac{1}{A^2}} = \frac{1 - A^2}{1}$$

→ A

→ B
↳ v (wrt A)

→ C
↳ w' (wrt B)

① $x' = \omega' t'$ → where does that come from

② $\omega = \frac{x}{t} = \frac{\gamma(x' + vt')}{\gamma\left[\frac{1}{v}\left(1 - \frac{1}{\gamma^2}\right)x' + t'\right]}$

$= \frac{\omega' t' + vt'}{\frac{1}{v}\left(1 - \frac{1}{\gamma^2}\right)\omega' t' + t'}$

$= \frac{\omega' + v}{\frac{1}{v}\left(1 - \frac{1}{\gamma^2}\right)\omega' + 1}$

Now I am going to rewrite γ as $\gamma(v)$ to specify that it depends on v .

$\omega = \frac{\omega' + v}{\frac{1}{v}\left(1 - \frac{1}{\gamma^2(v)}\right)\omega' + 1}$

Now we want to see everything from observer C's perspective.

To observer B, C is moving with vel w'

→ A
→ B
↳ v (w.r.t. to A)
→ C
↳ w' (w.r.t. to B)

$\begin{cases} x'' = \gamma(w') [x' - \omega' t'] & \textcircled{1} \\ x' = \gamma(w') [x'' + \omega' t''] & \textcircled{2} \end{cases}$

①: $\frac{x'}{\gamma} - \omega' t'' = x''$

~~②~~ ① = ①

also $x' = -vt'$ → how did that come about?

$$\frac{x'}{\gamma} - \omega' t'' = \gamma (x' - \omega' t')$$

$$\frac{x'}{\gamma} - \gamma x' + \gamma \omega' t' = \omega' t''$$

$$\gamma \left[\left(\frac{1}{\gamma^2} - 1 \right) x' + \omega' t' \right] = \omega' t''$$

$$\gamma \left[\frac{1}{\omega'} \left(\frac{1}{\gamma^2} - 1 \right) x' + t' \right] = t''$$

$$-\omega = \frac{x''}{t''} = \frac{\gamma [x' - \omega' t']}{\gamma \left[\frac{1}{\omega'} \left(\frac{1}{\gamma^2} - 1 \right) x' + t' \right]}$$

$$= \frac{-vt' - \omega' t'}{\frac{1}{\omega'} \left(\frac{1}{\gamma^2} - 1 \right) (-vt') + t'}$$

$$= \frac{-(v + \omega')}{\frac{1}{\omega'} \left(1 - \frac{1}{\gamma^2} \right) v + 1}$$

so

$$\omega = \frac{v + \omega'}{\frac{1}{\omega'} \left(1 - \frac{1}{\gamma^2} \right) v + 1}$$

A moving at
-v w.r.t to

B

a point x' man

Now, to verify that γ depends on w' .

|| rewrite w as

$$w = \frac{v + w'}{\frac{1}{w'} \left(1 - \frac{1}{\gamma^2(w')} \right) v + 1}$$

$$\text{Since } w = \frac{v + w'}{\frac{1}{w'} \left(1 - \frac{1}{\gamma^2(w)} \right) v + 1} = \frac{v + w'}{\frac{1}{v} \left(1 - \frac{1}{\gamma^2(v)} \right) w' + 1}$$

$$\text{that } \frac{v}{w'} \left(1 - \frac{1}{\gamma^2(w')} \right) = \frac{w'}{v} \left(1 - \frac{1}{\gamma^2(v)} \right)$$

$$\frac{\cancel{v} w'}{w'^2} \left(1 - \frac{1}{\gamma^2(w')} \right) = \frac{\cancel{v} w'}{v^2} \left(1 - \frac{1}{\gamma^2(v)} \right)$$

$$\underbrace{\frac{1}{w'^2} \left(1 - \frac{1}{\gamma^2(w')} \right)}_{\textcircled{1}} = \underbrace{\frac{1}{v^2} \left(1 - \frac{1}{\gamma^2(v)} \right)}_{\textcircled{2}} = B.$$

That means the two can't depend on time,
so we can set it to be a constant.

(

$$\omega = \frac{v + \omega'}{B\omega'v + 1}$$

we could have $\begin{cases} B=0 : \text{galilean} \\ B>1 : \text{relativistic} \end{cases}$

$$B = \frac{1}{v^2} \left(1 - \frac{1}{\gamma^2} \right)$$

$$v^2 B = 1 - \frac{1}{\gamma^2}$$

$$\gamma^2 v^2 B = \gamma^2 - 1$$

$$\gamma^2 [v^2 B - 1] = -1$$

$$\gamma^2 = \frac{1}{1 - v^2 B}$$

$$\gamma = \frac{1}{\sqrt{1 - v^2 B}}$$

turn out that $B = \frac{1}{c^2}$

$$\text{so } \gamma = \frac{1}{\sqrt{1 - \frac{v^2}{c^2}}}$$

Fiteau's
experiment

measured
yields

$$B = 1.1 \times 10^{-17} \text{ s}^2/\text{m}^2$$

→ Hence we have the Lorentz transformation:

$$\begin{cases} x' = \frac{1}{\sqrt{1-\frac{v^2}{c^2}}} (x - vt) \\ x = \frac{1}{\sqrt{1-\frac{v^2}{c^2}}} (x' + vt') \end{cases} \quad \begin{aligned} &1 - \frac{1}{1-\frac{v^2}{c^2}} \\ &\frac{x - \frac{v^2}{c^2}x}{1 - \frac{v^2}{c^2}} \end{aligned}$$

$$\begin{cases} t = \gamma \left[\frac{1}{v} \left(1 - \frac{1}{\gamma^2} \right) x' + t' \right] \\ = \frac{1}{\sqrt{1-\frac{v^2}{c^2}}} \left[\frac{1}{v} \left[x - x + \frac{v^2}{c^2} \right] x' + t' \right] \\ = \frac{1}{\sqrt{1-\frac{v^2}{c^2}}} \left[\frac{v}{c^2} x' + t' \right] \end{cases}$$

$$\begin{aligned} t' &= \gamma \left[\frac{1}{v} \left(\frac{1}{\gamma^2} - 1 \right) x + t \right] \\ &= \frac{1}{\sqrt{1-\frac{v^2}{c^2}}} \left[\frac{1}{v} \left[x - \frac{v^2}{c^2} x \right] x + t \right] \\ &= \frac{1}{\sqrt{1-\frac{v^2}{c^2}}} \left(-\frac{v}{c^2} x + t \right) \end{aligned}$$

□ Lorentz Transformation